pcuic/theories/TemplateToPCUICCorrectness.v
@@ -363,7 +363,7 @@ Proof.
   rewrite !Template.UnivSubst.subst_instance_constr_it_mkProd_or_LetIn in Hdecomp.
   rewrite !trans_it_mkProd_or_LetIn in Hdecomp.
   assert (#|Template.Ast.ind_params mdecl| =
-    #|PCUICSubstitution.subst_context
+    #|PCUICTyping.subst_context
       (inds (inductive_mind ind) u (map trans_one_ind_body (Template.Ast.ind_bodies mdecl))) 0
       (map trans_decl (Template.UnivSubst.subst_instance_context u (Template.Ast.ind_params mdecl)))|).
   now rewrite PCUICSubstitution.subst_context_length map_length Template.UnivSubst.subst_instance_context_length.
